function method

src/linear/layer1/List.dfy
@@ -9,11 +9,11 @@ trait ListIterator<A> {
     reads this, Parent(), Parent().Repr()
     ensures Valid() ==> Parent().Valid() && this in Parent().Iterators()
 
-  function Index(): nat
+  function Index(): int
     reads this, Parent(), Parent().Repr()
     requires Valid()
     requires Parent().Valid()
-    ensures Index() <= |Parent().Model()|
+    ensures -1 <= Index() <= |Parent().Model()|
 
   predicate HasNext?() 
     reads this, Parent(), Parent().Repr()
@@ -41,7 +41,33 @@ trait ListIterator<A> {
     ensures forall it | it in old(Parent().Iterators()) && old(it.Valid()) ::
       it.Valid() && it.Parent() == old(it.Parent()) && it.Index() == old(it.Index())
 
-  method Next() returns (x: A)
+  predicate HasPrev?() 
+    reads this, Parent(), Parent().Repr()
+    requires Valid()
+    requires Parent().Valid()
+  {  0 <= Index() }
+
+  method HasPrev() returns (b:bool) 
+    modifies this, Parent(), Parent().Repr()
+    requires allocated(Parent())
+    requires allocated(Parent().Repr())
+    ensures fresh(Parent().Repr()-old(Parent().Repr()))
+    ensures allocated(Parent().Repr())
+
+    requires Valid()
+    requires Parent().Valid()
+    ensures Valid()
+    ensures Parent().Valid()
+    ensures Parent() == old(Parent())
+    ensures Parent().Model() == old(Parent().Model()) 
+    ensures Index()==old(Index())
+    ensures b == HasPrev?()
+
+    ensures Parent().Iterators() >= old(Parent().Iterators())
+    ensures forall it | it in old(Parent().Iterators()) && old(it.Valid()) ::
+      it.Valid() && it.Parent() == old(it.Parent()) && it.Index() == old(it.Index())
+
+  method Next() 
     modifies this, Parent(), Parent().Repr()
     requires allocated(Parent())
     requires allocated(Parent().Repr())
@@ -57,8 +83,27 @@ trait ListIterator<A> {
     ensures Parent().Model() == old(Parent().Model())  
 
     ensures Parent().Iterators() >= old(Parent().Iterators())
-    ensures x == Parent().Model()[old(Index())]
     ensures Index() == 1 + old(Index())
+    ensures forall it | it in old(Parent().Iterators()) && old(it.Valid()) ::
+      it.Valid() && it.Parent()==old(it.Parent()) && (it != this ==> it.Index() == old(it.Index()))
+  
+  method Prev() 
+    modifies this, Parent(), Parent().Repr()
+    requires allocated(Parent())
+    requires allocated(Parent().Repr())
+    ensures fresh(Parent().Repr()-old(Parent().Repr()))
+    ensures allocated(Parent().Repr())
+
+    requires Valid()
+    requires Parent().Valid()
+    requires HasPrev?()
+    ensures Valid()
+    ensures Parent().Valid()
+    ensures Parent() == old(Parent())  
+    ensures Parent().Model() == old(Parent().Model())  
+
+    ensures Parent().Iterators() >= old(Parent().Iterators())
+    ensures Index() + 1 == old(Index())
     ensures forall it | it in old(Parent().Iterators()) && old(it.Valid()) ::
       it.Valid() && it.Parent()==old(it.Parent()) && (it != this ==> it.Index() == old(it.Index()))
   
@@ -71,7 +116,7 @@ trait ListIterator<A> {
 
     requires Valid()
     requires Parent().Valid()
-    requires HasNext?()
+    requires HasNext?() && HasPrev?()
     ensures Valid()
     ensures Parent().Valid()
     ensures Parent() == old(Parent())  
@@ -115,7 +160,7 @@ trait ListIterator<A> {
 
     requires Valid()
     requires Parent().Valid()
-    requires HasNext?()
+    requires HasNext?() && HasPrev?()
     ensures Valid()
     ensures Parent().Valid()
     ensures Parent() == old(Parent())
@@ -272,6 +317,7 @@ trait List<A> extends ADT<seq<A>> {
     requires mid.Valid()
     requires mid.Parent() == this
     requires mid in Iterators()
+    requires mid.HasPrev?()
     ensures Valid()
     ensures Model() == Seq.Insert(x, old(Model()), old(mid.Index()))
 
@@ -290,7 +336,7 @@ trait List<A> extends ADT<seq<A>> {
     requires Valid()
     requires mid.Valid()
     requires mid.Parent() == this
-    requires mid.HasNext?()
+    requires mid.HasNext?() && mid.HasPrev?()
     requires mid in Iterators()
     ensures Valid()
     ensures Model() == Seq.Remove(old(Model()), old(mid.Index()))
